\chapter{Future Logic Collusion Formula Examples}
\label{app:FutureLogicCollusionFormulaExamples}

The following examples evaluate the collusion formula exressed in future logic from chapter \ref{chap:Monitoring For Security Properties} over two traces using the LTL semantics in defintions \ref{def:FutureEmptyTraceSemantics} and \ref{def:FutureNon-emptyTraceSemantics}, from chapter \ref{chap:Linear Temporal Logic}.  The first example evaluates the formula over a trace that satisfies the formula, while the second example is a trace where the receive event is before the send event, therefore it does not satisfy the formula. 

\begin{myEx} Future Logic Collusion Formula Over a Positive Trace\\

\noindent
$\varphi = \LTLeventually(q \land \LTLeventually(s \land \LTLeventually(r \land \LTLeventually p)))$\\
$t = \langle q, s, r, p \rangle$\\

\begin{enumerate}
\item $\langle q,s,r,p \rangle \Vdash \LTLeventually(q \land \LTLeventually(s \land \LTLeventually(r \land \LTLeventually p)))$, root formula.\\ % 1 

\item $q, \langle s,r,p \rangle \Vdash q \land \LTLeventually(s \land \LTLeventually(r \land \LTLeventually p))$ or $\langle s,r,p \rangle \Vdash \LTLeventually(q \land \LTLeventually(s \land \LTLeventually(r \land \LTLeventually p)))$, by rule 17 applied to step 1.\\ %2

\item $q , \langle s,r,p \rangle \Vdash q \land \LTLeventually(s \land \LTLeventually(r \land \LTLeventually p))$, left formula from step 2.\\ % 3

\item $q , \langle s,r,p \rangle \Vdash q$\ and\ $q , \langle s,r,p \rangle \Vdash \LTLeventually(s \land \LTLeventually(r \land \LTLeventually p))$, by rule 13 applied to step 3.\\ % 4

\item $q , \langle s,r,p \rangle \Vdash q$, left formula from step 4.\\ % 5

\item $q , \langle s,r,p \rangle \Vdash q = \top$, by rule 10 applied to step 5.\\ % 6

\item $q, \langle s,r,p \rangle \Vdash \LTLeventually(s \land \LTLeventually(r \land \LTLeventually p))$, right formula from step 4.\\ % 7

\item $q, \langle s,r,p \rangle \Vdash s \land \LTLeventually(r \land \LTLeventually p)$ or $\langle s,r,p \rangle \Vdash \LTLeventually(s \land \LTLeventually(r \land \LTLeventually p))$, by rule 17 applied to step 7.\\ %8

\item $q, \langle s,r,p \rangle \Vdash s \land \LTLeventually(r \land \LTLeventually p)$, left formula from step 8.\\ %9

\item $q, \langle s,r,p \rangle \Vdash s$ and $q, \langle s,r,p \rangle \Vdash \LTLeventually(r \land \LTLeventually p)$, by rule 13 applied to step 9.\\ % 10

\item $q, \langle s,r,p \rangle \Vdash s$, left formula from step 10.\\ % 11

\item $q, \langle s,r,p \rangle \Vdash s = \bot$, by rule 10 applied to step 11.\\ % 12

\item $\langle s,r,p \rangle \Vdash \LTLeventually(s \land \LTLeventually(r \land \LTLeventually p))$, right formula from step 8.\\ %13

\item $s, \langle r,p \rangle \Vdash s \land \LTLeventually(r \land \LTLeventually p)$ or $\langle r,p \rangle \Vdash \LTLeventually(s \land \LTLeventually(r \land \LTLeventually p))$, by rule 17 applied to step 13.\\ % 14

\item $s, \langle r,p \rangle \Vdash s \land \LTLeventually(r \land \LTLeventually p)$, left formula from step 14.\\ % 15

\item $s, \langle r,p \rangle \Vdash s$ and $s, \langle r,p \rangle \Vdash \LTLeventually(r \land \LTLeventually p)$, by rule 13 applied to step 15.\\ % 16

\item $s, \langle r,p \rangle \Vdash s$, left formula from step 16.\\ % 17

\item $s, \langle r,p \rangle \Vdash s = \top$, by rule 10 applied to step 17.\\ % 18

\item $s, \langle r,p \rangle \Vdash \LTLeventually(r \land \LTLeventually p)$, right formula from step 16.\\ % 19

\item $s, \langle r,p \rangle \Vdash r \land \LTLeventually p$ or $\langle r,p \rangle \Vdash \LTLeventually(r \land \LTLeventually p)$, by rule 17 applied to step 19\\ % 20

\item $s, \langle r,p \rangle \Vdash r \land \LTLeventually p$, left formula from step 20.\\ % 21

\item $s, \langle r,p \rangle \Vdash r$ and $s, \langle r,p \rangle \Vdash \LTLeventually p$, by rule 13 applied to step 21.\\ % 22

\item $s, \langle r,p \rangle \Vdash r$, left formula from step 22.\\ % 23

\item $s, \langle r,p \rangle \Vdash r = \bot$, by rule 10 applied to step 23\\ % 24

\item $\langle r,p \rangle \Vdash \LTLeventually(r \land \LTLeventually p)$, right formula from step 20.\\ % 25

\item $r, \langle p \rangle \Vdash r \land \LTLeventually p$ or $\langle p \rangle \Vdash \LTLeventually(r \land \LTLeventually p)$, by rule 17 applied to step 25.\\ % 26

\item $r, \langle p \rangle \Vdash r \land \LTLeventually p$, left forumla from step 25.\\ % 27

\item $r, \langle p \rangle \Vdash r$ and $r, \langle p \rangle \Vdash \LTLeventually p$, by rule 13 applied to step 27.\\ % 28

\item $r, \langle p \rangle \Vdash r$, left formula from step 28.\\ % 29

\item $r, \langle p \rangle \Vdash r = \top$, by rule 10 applied to step 29.\\ % 30

\item $r, \langle p \rangle \Vdash \LTLeventually p$, right formula from step 28.\\ % 31

\item $r, \langle p \rangle \Vdash p$ or $\langle p \rangle \Vdash \LTLeventually p$, by rule 17 applied to step 31.\\ % 32

\item $r, \langle p \rangle \Vdash p$, left formula from step 32.\\ % 33

\item $r, \langle p \rangle \Vdash p = \bot$, by rule 10 applied to step 33.\\ % 34

\item $\langle p \rangle \Vdash \LTLeventually p$, right formula from step 32.\\ % 35

\item $p, \langle \rangle \Vdash p$ or $ \langle \rangle \Vdash \LTLeventually p$, by rule 17 applied to step 35.\\ % 36

\item $p, \langle \rangle \Vdash p$, left formula from step 36.\\ % 37

\item $p, \langle \rangle \Vdash p = \top$, by rule 10 applied to step 37.% 38
\end{enumerate}
\qed
\end{myEx}

\begin{myEx} Future Logic Collusion Formula Over a Negative Trace\\

\noindent
$\varphi = \LTLeventually(q \land \LTLeventually(s \land \LTLeventually(r \land \LTLeventually p)))$\\
$t = \langle q, r, s, p \rangle$

\begin{enumerate}
\item $\langle q,r,s,p \rangle \Vdash \LTLeventually(q \land \LTLeventually(s \land \LTLeventually(r \land \LTLeventually p)))$, root formula.\\ % 1 

\item $q, \langle r,s,p \rangle \Vdash q \land \LTLeventually(s \land \LTLeventually(r \land \LTLeventually p))$ or $\langle r,s,p \rangle \Vdash \LTLeventually(q \land \LTLeventually(s \land \LTLeventually(r \land \LTLeventually p)))$, by rule 17 applied to step 1.\\ % 2

\item $q, \langle r,s,p \rangle \Vdash q \land \LTLeventually(s \land \LTLeventually(r \land \LTLeventually p))$, left formula from step2.\\ % 3

\item $q, \langle r,s,p \rangle \Vdash q$ and $q, \langle r,s,p \rangle \Vdash \LTLeventually(s \land \LTLeventually(r \land \LTLeventually p))$, by rule 13 applied to step 3.\\ % 4

\item $q, \langle r,s,p \rangle \Vdash q$, left formula from step 4.\\ % 5

\item $q, \langle r,s,p \rangle \Vdash q = \top$, by rule 10 applied to step 5.\\ % 6

\item $q, \langle r,s,p \rangle \Vdash \LTLeventually(s \land \LTLeventually(r \land \LTLeventually p))$, right formula from step 4.\\ % 7

\item $q, \langle r,s,p \rangle \Vdash s \land \LTLeventually(r \land \LTLeventually p)$ or $\langle r,s,p \rangle \Vdash \LTLeventually(s \land \LTLeventually(r \land \LTLeventually p))$, by rule 17 applied to step 7.\\ % 8

\item $q, \langle r,s,p \rangle \Vdash s \land \LTLeventually(r \land \LTLeventually p)$, left formula from step 8.\\ % 9

\item $q, \langle r,s,p \rangle \Vdash s$ and $q, \langle r,s,p \rangle \Vdash \LTLeventually(r \land \LTLeventually p)$, by rule 13 applied to step 9.\\ % 10

\item $q, \langle r,s,p \rangle \Vdash s$, left formula from step 10.\\ % 11

\item $q, \langle r,s,p \rangle \Vdash s = \bot$, by rule 10 applied to step 11.\\ % 12

\item $\langle r,s,p \rangle \Vdash \LTLeventually(s \land \LTLeventually(r \land \LTLeventually p))$, right formula from step 8.\\ % 13

\item $r, \langle s,p \rangle \Vdash s \land \LTLeventually(r \land \LTLeventually p)$ or $\langle s,p \rangle \Vdash \LTLeventually(s \land \LTLeventually(r \land \LTLeventually p))$, by rule 17 applied to step 13.\\ % 14

\item $r, \langle s,p \rangle \Vdash s \land \LTLeventually(r \land \LTLeventually p)$, left formula from step 14.\\ % 15

\item $r, \langle s,p \rangle \Vdash s$ and $r, \langle s,p \rangle \Vdash \LTLeventually(r \land \LTLeventually p)$, by rule 13 applied to step 15.\\ % 16

\item $r, \langle s,p \rangle \Vdash s$, left formula from step 16.\\ % 17

\item $r, \langle s,p \rangle \Vdash s = \bot$, by rule 10 applied to step 17.\\ % 18

\item $\langle s,p \rangle \Vdash \LTLeventually(s \land \LTLeventually(r \land \LTLeventually p))$, right formula from step 14.\\ % 19

\item $s, \langle p \rangle \Vdash s \land \LTLeventually(r \land \LTLeventually p)$ or $\langle p \rangle \Vdash \LTLeventually(s \land \LTLeventually(r \land \LTLeventually p))$, by rule 17 applied to step 19.\\ % 20

\item $s, \langle p \rangle \Vdash s \land \LTLeventually(r \land \LTLeventually p)$, left formula from step 20.\\ % 21

\item $s, \langle p \rangle \Vdash s$ and $s, \langle p \rangle \Vdash \LTLeventually(r \land \LTLeventually p)$, by rule 13 applied to step 21.\\ % 22

\item $s, \langle p \rangle \Vdash s$, left formula from step 22.\\ % 23

\item $s, \langle p \rangle \Vdash s = \top$, by rule 10 applied to step 23.\\ % 24

\item $s, \langle p \rangle \Vdash \LTLeventually(r \land \LTLeventually p)$, right formula from step 22.\\ % 25

\item $s, \langle p \rangle \Vdash r \land \LTLeventually p$ or $\langle p \rangle \Vdash \LTLeventually(r \land \LTLeventually p)$, by rule 17 applied to step 25.\\ % 26

\item $s, \langle p \rangle \Vdash r \land \LTLeventually p$, left formula from step 26.\\ % 27

\item $s, \langle p \rangle \Vdash r$ and $s, \langle p \rangle \Vdash \LTLeventually p$, by rule 13 applied to step 27.\\ % 28

\item $s, \langle p \rangle \Vdash r$ left formula from step 28.\\ % 29

\item $s, \langle p \rangle \Vdash r = \bot$, by rule 10 applied to step 29.\\ % 30

\item $\langle p \rangle \Vdash \LTLeventually(r \land \LTLeventually p)$, right formula from step 26.\\ % 31

\item $p, \langle \rangle \Vdash r \land \LTLeventually p$ or $\langle \rangle \Vdash \LTLeventually(r \land \LTLeventually p)$\\ % 32

\item $p, \langle \rangle \Vdash r \land \LTLeventually p$, by rule 17 applied to step 32.\\ % 33

\item $p, \langle \rangle \Vdash r$ and $p, \langle \rangle \Vdash \LTLeventually p$, by rule 13 applied to step 33.\\ % 34

\item $p, \langle \rangle \Vdash r$, left formula from step 34.\\ % 35

\item $p, \langle \rangle \Vdash r = \bot$, by rule 10 applied to step 35.\\ % 36

\item $\langle \rangle \Vdash \LTLeventually(r \land \LTLeventually p)$, right formula from step 32.\\ % 37

\item $\langle \rangle \Vdash r \land \LTLeventually p$, by rule 8 applied to step 37.\\ % 38
 
\item $\langle \rangle \Vdash r$ and $\langle \rangle \Vdash \LTLeventually p$, by rule 4 applied to step 38.\\ % 39

\item $\langle \rangle \Vdash r$, left formula from step 39\\ % 40

\item $\langle \rangle \Vdash r = \bot$, by rule 1 applied to step 40.\\% 42
\end{enumerate}
\qed
\end{myEx}