\chapter{Past Logic Collusion Formula Examples}
\label{app:PastLogicCollusionFormulaExamples}

The following examples evaluate the collusion formula expressed in past logic from chapter \ref{chap:Reverse Rosu-Havelund Algorithm} over two traces using the LTL semantics in defintions \ref{def:PastEmptyTraceSemantics} and \ref{def:PastNon-emptyTraceSemantics}, from chapter \ref{chap:Linear Temporal Logic}.  The first example evaluates the formula over a trace that satisfies the formula, while the second example is a trace where the send and receive events are reverse so that the receive is before the send event, therefore it does not satisfy the formula. 

\begin{myEx} Past Logic Collusion Formula Over a Positive Trace\\

\noindent
$\varphi = \LTLonce(p \land \LTLonce(r \land \LTLonce(s \land \LTLonce q)))$\\
$t = \langle q, s, r, p \rangle$\\

\begin{enumerate}
\item $\langle q,s,r,p \rangle \Vdash \LTLonce(p \land \LTLonce(r \land \LTLonce(s \land \LTLonce q)))$, root formula.\\ % 1.

\item $\langle q,s,r \rangle, p \Vdash p \land \LTLonce(r \land \LTLonce(s \land \LTLonce q))$ or $\langle q,s,r \rangle \Vdash \LTLonce(p \land \LTLonce(r \land \LTLonce(s \land \LTLonce q)))$, by rule 35 applied to step 1.\\ % 2

\item $\langle q,s,r \rangle, p \Vdash p \land \LTLonce(r \land \LTLonce(s \land \LTLonce q))$, left formula from step 2.\\ % 3

\item $\langle q,s,r \rangle, p \Vdash p$ and $\langle q,s,r \rangle, p \Vdash \LTLonce(r \land \LTLonce(s \land \LTLonce q))$, by rule 31 applied to step 3.\\ % 4

\item $\langle q,s,r \rangle, p \Vdash p$, left formula from step 4.\\ % 5

\item $\langle q,s,r \rangle, p \Vdash p = \top$, by rule 28 applied to step 5.\\ % 6

\item $\langle q,s,r \rangle, p \Vdash \LTLonce(r \land \LTLonce(s \land \LTLonce q))$, right formula from step 4.\\ % 7

\item $\langle q,s,r \rangle, p \Vdash r \land \LTLonce(s \land \LTLonce q)$ or $\langle q,s,r \rangle \Vdash \LTLonce(r \land \LTLonce(s \land \LTLonce q))$, by rule 35 applied to step 5.\\ % 8

\item $\langle q,s,r \rangle, p \Vdash r \land \LTLonce(s \land \LTLonce q)$, left formula from step 8.\\ % 9

\item $\langle q,s,r \rangle, p \Vdash r$ and $ \langle q,s,r \rangle, p \Vdash \LTLonce(s \land \LTLonce q)$, by rule 31 applied to step 9.\\ % 10

\item $\langle q,s,r \rangle, p \Vdash r$, left formula from step 10.\\ % 11

\item $\langle q,s,r \rangle, p \Vdash r = \bot$, by rule 28 applied to step 11.\\ % 12

\item $\langle q,s,r \rangle \Vdash \LTLonce(r \land \LTLonce(s \land \LTLonce q))$, right formula from step 8.\\ % 13

\item $\langle q,s \rangle, r \Vdash r \land \LTLonce(s \land \LTLonce q)$ or $\langle q,s \rangle \Vdash \LTLonce(r \land \LTLonce(s \land \LTLonce q))$, by rule 35 applied to step 13.\\ % 14

\item $\langle q,s \rangle, r \Vdash r \land \LTLonce(s \land \LTLonce q)$, left formula from step 14.\\ % 15

\item $\langle q,s \rangle, r \Vdash r$ and $\langle q,s \rangle, r \Vdash \LTLonce(s \land \LTLonce q)$, by rule 31 applied to step 15.\\ % 16

\item $\langle q,s \rangle, r \Vdash r$, left formula from step 16.\\ % 17

\item $\langle q,s \rangle, r \Vdash r = \top$, by rule 28 applied to step 17.\\ % 18

\item $\langle q,s \rangle, r \Vdash \LTLonce(s \land \LTLonce q)$, right formula from step 16.\\ % 19

\item $\langle q,s \rangle, r \Vdash s \land \LTLonce q$ or $\langle q,s \rangle \Vdash \LTLonce(s \land \LTLonce q)$, by rule 35 applied to step 19.\\ % 20

\item $\langle q,s \rangle, r \Vdash s \land \LTLonce q$, left formula from step 20.\\ % 21

\item $\langle q,s \rangle, r \Vdash s$ and $\langle q,s \rangle, r \Vdash \LTLonce q$, by rule 31 applied to step 21.\\ % 22

\item $\langle q,s \rangle, r \Vdash s$, left formula from step 22.\\ % 23

\item $\langle q,s \rangle, r \Vdash s = \bot$, by rule 28 applied to step 23.\\ % 24

\item $\langle q,s \rangle \Vdash \LTLonce(s \land \LTLonce q)$, right formula from step 20.\\ % 25

\item $\langle q \rangle, s \Vdash s \land \LTLonce q$ or $\langle q \rangle, s \Vdash \LTLonce(s \land \LTLonce q)$, by rule 35 applied to step 25.\\ % 26

\item $\langle q \rangle, s \Vdash s \land \LTLonce q$, left formula from step 26.\\ % 27

\item $\langle q \rangle, s \Vdash s$ and $\langle q \rangle, s \Vdash \LTLonce q$, by rule 31 applied to step 27.\\ % 28

\item $\langle q \rangle, s \Vdash s$, left formula from step 28.\\ % 29

\item $\langle q \rangle, s \Vdash s = \top$, by rule 28 applied to step 29.\\ % 30

\item $\langle q \rangle, s \Vdash \LTLonce q$, right formula from step 28.\\ % 31

\item $\langle q \rangle, s \Vdash q$ or $\langle q \rangle \Vdash \LTLonce q$, by rule 35 applied to step 31.\\ % 32

\item $\langle q \rangle, s \Vdash q$, left formula from step 32.\\ % 33

\item $\langle q \rangle, s \Vdash q = \bot$, by rule 28 applied to step 33.\\ % 34

\item $\langle q \rangle \Vdash \LTLonce q$, right formula from step 32.\\ % 35

\item $\langle \rangle, q \Vdash q$ or $\langle \rangle \Vdash \LTLonce q$, by rule 35 applied to step 35.\\ % 36

\item $\langle \rangle, q \Vdash q$, left formula from step 36.\\ % 37

\item $\langle \rangle, q \Vdash q = \top$, by rule 28 applied to step 37.\\ % 38
\end{enumerate}
\qed
\end{myEx}

\begin{myEx} Past Logic Collusion Formula Over a Negative Trace\\

\noindent
$\varphi = \LTLonce(p \land \LTLonce(r \land \LTLonce(s \land \LTLonce q)))$\\
$t = \langle q, r, s, p \rangle$\\

\begin{enumerate}
\item $\langle q, r, s, p \rangle \Vdash \LTLonce(p \land \LTLonce(r \land \LTLonce(s \land \LTLonce q)))$, root formula.\\ % 1

\item $\langle q, r, s \rangle, p \Vdash p \land \LTLonce(r \land \LTLonce(s \land \LTLonce q))$ or $\langle q, r, s \rangle \Vdash \LTLonce(p \land \LTLonce(r \land \LTLonce(s \land \LTLonce q)))$, by rule 35 applied to step 1.\\ % 2

\item $\langle q, r, s \rangle, p \Vdash p \land \LTLonce(r \land \LTLonce(s \land \LTLonce q))$, left formula from step 2.\\ % 3

\item $\langle q, r, s \rangle, p \Vdash p$ and $\langle q, r, s \rangle, p \Vdash \LTLonce(r \land \LTLonce(s \land \LTLonce q))$, by rule 31 applied to step 3.\\ % 4

\item $\langle q, r, s \rangle, p \Vdash p$, left formula from step 4.\\ % 5

\item $\langle q, r, s \rangle, p \Vdash p = \top$, by rule 28 applied to step 5.\\ % 6

\item $\langle q, r, s \rangle, p \Vdash \LTLonce(r \land \LTLonce(s \land \LTLonce q))$, right formula from step 4.\\ % 7

\item $\langle q, r, s \rangle, p \Vdash r \land \LTLonce(s \land \LTLonce q)$ or $\langle q, r, s \rangle \Vdash \LTLonce(r \land \LTLonce(s \land \LTLonce q))$, by rule 35 from step 7.\\ % 8

\item $\langle q, r, s \rangle, p \Vdash r \land \LTLonce(s \land \LTLonce q)$, left formula from step 8.\\ % 9

\item $\langle q, r, s \rangle, p \Vdash r$ and $\langle q, r, s \rangle, p \Vdash \LTLonce(s \land \LTLonce q)$, by rule 31 applied to step 9.\\ % 10

\item $\langle q, r, s \rangle, p \Vdash r$, left formula from step 10.\\ % 11

\item $\langle q, r, s \rangle, p \Vdash r = \bot$, by rule 28 applied to step 11.\\ % 12

\item $\langle q, r, s \rangle \Vdash \LTLonce(r \land \LTLonce(s \land \LTLonce q))$, right formula from step 8.\\ % 13

\item $\langle q, r \rangle, s \Vdash r \land \LTLonce(s \land \LTLonce q)$ or $\langle q, r \rangle \Vdash \LTLonce(r \land \LTLonce(s \land \LTLonce q))$, by rule 35 applied to step 13.\\ % 14

\item $\langle q, r \rangle, s \Vdash r \land \LTLonce(s \land \LTLonce q)$, left formula from step 14.\\ % 15

\item $\langle q, r \rangle, s \Vdash r$ and $\langle q, r \rangle, s \Vdash \LTLonce(s \land \LTLonce q)$, by rule 31 applied to step 15.\\ % 16

\item $\langle q, r \rangle, s \Vdash r$, left formula from step 16.\\ % 17

\item $\langle q, r \rangle, s \Vdash r = \bot$, by rule 28 applied to step 17.\\ % 18

\item $\langle q, r \rangle \Vdash \LTLonce(r \land \LTLonce(s \land \LTLonce q))$, right formula from step 14.\\ % 19

\item $\langle q \rangle, r \Vdash r \land \LTLonce(s \land \LTLonce q)$ or $\langle q \rangle \Vdash \LTLonce(r \land \LTLonce(s \land \LTLonce q))$, by rule 35 applied to step 19.\\ % 20

\item $\langle q \rangle, r \Vdash r \land \LTLonce(s \land \LTLonce q)$, left formula from step 20.\\ % 21

\item $\langle q \rangle, r \Vdash r$ and $\langle q \rangle, r \Vdash \LTLonce(s \land \LTLonce q)$, by rule 31 applied to step 21.\\ % 22

\item $\langle q \rangle, r \Vdash r$, left formula from step 22.\\ % 23

\item $\langle q \rangle, r \Vdash r = \top$, by rule 28 applied to step 23.\\ % 24

\item $\langle q \rangle, r \Vdash \LTLonce(s \land \LTLonce q)$, right formula from step 22.\\ % 25

\item $\langle q \rangle, r \Vdash s \land \LTLonce q$ or $\langle q \rangle \Vdash \LTLonce(s \land \LTLonce q)$, by rule 35 applied to step 25.\\ % 26

\item $\langle q \rangle, r \Vdash s \land \LTLonce q$, left formula from step 26.\\ % 27

\item $\langle q \rangle, r \Vdash s$ and $\langle q \rangle, r \Vdash \LTLonce q$, by rule 31 applied to step 27.\\ % 28

\item $\langle q \rangle, r \Vdash s$, left formula from step 28.\\ % 29

\item $\langle q \rangle, r \Vdash s = \bot$, by rule 28 applied to step 29.\\ % 30

\item $\langle q \rangle \Vdash \LTLonce(s \land \LTLonce q)$, right formula from step 26.\\ % 31

\item $\langle \rangle, q \Vdash s \land \LTLonce q$ or $\langle \rangle \Vdash \LTLonce(s \land \LTLonce q)$, by rule 35 applied to step 31.\\ % 32

\item $\langle \rangle, q \Vdash s \land \LTLonce q$, left formula from step 32.\\ % 33

\item $\langle \rangle, q \Vdash s$ and $\langle \rangle, q \Vdash \LTLonce q$, by rule 31 applied to step 33.\\ % 34

\item $\langle \rangle, q \Vdash s$, left formula from step 34.\\ % 35

\item $\langle \rangle, q \Vdash s = \bot$, by rule 28 applied to step 35.\\ % 36

\item $\langle \rangle \Vdash \LTLonce(s \land \LTLonce q)$, right formula from step 32.\\ % 37

\item $\langle \rangle \Vdash s \land \LTLonce q$, by rule 26 applied to step 37.\\ % 38

\item $\langle \rangle \Vdash s$ and $\langle \rangle \Vdash \LTLonce q$, by rule 22 applied to step 38.\\ % 39

\item $\langle \rangle \Vdash s$, left formula from step 39.\\ % 40

\item $\langle \rangle \Vdash s = \bot$, by rule 19 applied to step 40.\\ % 41
\end{enumerate}
\qed
\end{myEx}
